----------------------------------------------------------------------
 Committing in the wordFunctor.sml file of the n_bit library.

This has now been modified to use the new higher order quotients
library instead of EquivType.

The source code involved a good deal of messy probing into the
internals of the quotient operation, which was dependent on the
previous implementation.  This has been clarified, but the current
file is now dependent somewhat on the implementation of the new
quotient library, and so would not be expected to build if the
references to open "quotient" were changed to open "EquivType".

There were several places where the source code manually dealt
with the Hilbert choice operator, also referred to as the "SELECT"
operator.  These have been elided, since the new quotient package
provides an encapsulation of these details.  Many proofs have been
simplified or eliminated.  In particular, the tactic "SELECT_WORD_TAC"
has been changed to the simpler "QUOTIENT_WORD_TAC", which is used
repeatedly.

This completes the set of modifications to parts of the standard
HOL system that used EquivType.  I will also examine the examples
directory to see if there are any dependencies there.

 Modified Files:
 	hol98/src/n_bit/wordFunctor.sml
 ----------------------------------------------------------------------

src/n_bit/wordFunctor.sml
@@ -2,12 +2,12 @@ functor wordFunctor (val bits : int) =
 struct
 
 (*
-   app load ["EquivType","pairTheory", "metisLib",
+   app load ["quotient","pairTheory", "metisLib",
              "numeralTheory","wordUtil","bitsTheory","numeral_bitsTheory"];
 val bits = 8;
 *)
 
-open HolKernel boolLib wordUtil Q Parse EquivType
+open HolKernel boolLib wordUtil Q Parse quotient
      computeLib bossLib simpLib numLib pairTheory numeralTheory
      arithmeticTheory prim_recTheory bitsTheory metisLib;
 
@@ -47,6 +47,7 @@ val EQUIV_QT = prove(
     THEN B_RW_TAC [FUN_EQ_THM,EQUIV_def,MOD_WL_def]
 );
 
+val EQUIV_REFL = PROVE [EQUIV_QT] `!x. x == x`;
 val EQUIV_SYM = PROVE [EQUIV_QT] `!x y. x == y = y == x`;
 
 (* -------------------------------------------------------- *)
@@ -577,18 +578,19 @@ val bool_not = Term`$~`
 val _ = overload_on ("~", Term`$word_2comp`);
 val _ = overload_on ("~", bool_not);
 
-val mk_word    = prim_mk_const {Name = "mk_word"^sbits,  Thy = "word"^sbits};
-val dest_word  = prim_mk_const {Name = "dest_word"^sbits,Thy = "word"^sbits};
+val mk_word    = prim_mk_const {Name = "word"^sbits^"_ABS",Thy = "word"^sbits};
+val dest_word  = prim_mk_const {Name = "word"^sbits^"_REP",Thy = "word"^sbits};
 (*val word_ty_aq = ty_antiq (mk_type ("word"^sbits, []));*)
 
-val n2w_def = Define `n2w n = ^mk_word ($== n)`;
-val w2n_def = Define `w2n w = MOD_WL ($@ (^dest_word w))`;
+val n2w_def = Define `n2w n = ^mk_word n`;
+val w2n_def = Define `w2n w = MOD_WL (^dest_word w)`;
 
 val _ = add_bare_numeral_form (#"w", SOME "n2w");
 
-val word_tybij = definition ("word"^sbits^"_tybij");
-val mk_word_one_one  = BETA_RULE (prove_abs_fn_one_one word_tybij);
-val word_abs_fn_onto = BETA_RULE (prove_abs_fn_onto word_tybij);
+val word_QUOTIENT = REWRITE_RULE [quotientTheory.QUOTIENT_def,EQUIV_REFL]
+                     (definition ("word"^sbits^"_QUOTIENT"));
+val mk_word_one_one  = GSYM (CONJUNCT2 word_QUOTIENT);
+val word_abs_fn_onto = CONJUNCT1 word_QUOTIENT;
 
 val word_L_def = save_thm("word_L_def",REWRITE_RULE [GSYM n2w_def] (definition "word_L_def"));
 val word_H_def = save_thm("word_H_def",REWRITE_RULE [GSYM n2w_def] (definition "word_H_def"));
@@ -913,44 +915,18 @@ val FORALL_WORD = store_thm("FORALL_WORD",
 
 val EQUIV_EXISTS = prove(`!y. ?x. $== y = $== x`, PROVE_TAC []);
 
-(* |- (mk_word ($== x) = mk_word ($== y)) = ($== x = $== y) *)
-val mk_word_eq_one_one = SIMP_RULE bool_ss [EQUIV_EXISTS] (SPECL [`$== x`,`$== y`] mk_word_one_one);
-
-val dest_word_mk_word_eq = prove(
-  `!a. ^dest_word (^mk_word ($== a)) = $== a`,
-  STRIP_TAC THEN REWRITE_TAC [EQUIV_EXISTS,GSYM (BETA_RULE word_tybij)]
-);
-
-val dest_word_mk_word_eq2 = prove(
-  `!a x. (^dest_word (^mk_word ($== a)) x) = (a == x)`,
-  STRIP_TAC THEN REWRITE_TAC [dest_word_mk_word_eq]
-);
-
-val dest_word_mk_word_exists = prove(
-  `?x. ^dest_word (^mk_word ($== a)) x`,
-  B_RW_TAC [dest_word_mk_word_eq2,EQUIV_def] THEN PROVE_TAC []
-);
-
 (* -------------------------------------------------------- *)
-
-val etar = prove(
-  `!p:num -> bool. $@p = @x. p x`,
-  GEN_TAC THEN CONV_TAC (ONCE_DEPTH_CONV ETA_CONV) THEN PROVE_TAC []
-);
 
 val MOD_WL_ELIM = store_thm("MOD_WL_ELIM",
   `!n. n2w (MOD_WL n) = n2w n`,
-  B_RW_TAC [n2w_def,mk_word_eq_one_one]
-    THEN ONCE_REWRITE_TAC [FUN_EQ_THM]
-    THEN REWRITE_TAC [EQUIV_def,MOD_WL_IDEM2]
+  B_RW_TAC [n2w_def,mk_word_one_one]
+    THEN REWRITE_TAC [MOD_WL_QT]
 );
 
 val w2n_EVAL = store_thm("w2n_EVAL",
   `!n. w2n (n2w n) = MOD_WL n`,
   B_RW_TAC [w2n_def,n2w_def]
-    THEN ONCE_REWRITE_TAC [etar] THEN SELECT_ELIM_TAC
-    THEN B_RW_TAC [dest_word_mk_word_exists,dest_word_mk_word_eq2]
-    THEN B_FULL_SIMP_TAC [EQUIV_def]
+    THEN REWRITE_TAC [GSYM EQUIV_def, word_QUOTIENT]
 );
 
 fun Cases_on_word tm = STRUCT_CASES_TAC (SPEC tm word_nchotomy);
@@ -964,10 +940,8 @@ val w2n_ELIM = store_thm("w2n_ELIM",
 
 val n2w_11 = store_thm("n2w_11",
   `!a b. (n2w a = n2w b) = (MOD_WL a = MOD_WL b)`,
-  REPEAT STRIP_TAC
-    THEN Cases_on_word `a`
-    THEN Cases_on_word `b`
-    THEN REWRITE_TAC [n2w_def,mk_word_eq_one_one,EQUIV_QT,GSYM EQUIV_def]
+  REPEAT GEN_TAC
+    THEN REWRITE_TAC [n2w_def,mk_word_one_one,GSYM EQUIV_def]
 );
 
 val w2n_n2w = store_thm("w2n_n2w",
@@ -994,29 +968,26 @@ val w2n_LT = store_thm("w2n_LT",
 
 (* -------------------------------------------------------- *)
 
-fun SELECT_WORD_TAC th1 th2 =
-  B_SIMP_TAC [n2w_def,th1,mk_word_eq_one_one]
-    THEN ONCE_REWRITE_TAC [etar]
+fun QUOTIENT_WORD_TAC th1 th2 =
+  B_SIMP_TAC [n2w_def,th1,mk_word_one_one]
     THEN REPEAT STRIP_TAC
-    THEN REPEAT SELECT_ELIM_TAC
-    THEN B_RW_TAC [dest_word_mk_word_exists,dest_word_mk_word_eq2]
-    THEN ASM_B_SIMP_TAC [th2,EQUIV_SYM,GSYM EQUIV_QT];
+    THEN ASM_B_SIMP_TAC [th2,word_QUOTIENT];
 
 val ADD_EVAL = store_thm("ADD_EVAL",
   `!a b. n2w a + n2w b = n2w (a + b)`,
-  SELECT_WORD_TAC word_add_def ADD_WELLDEF);
+  QUOTIENT_WORD_TAC word_add_def ADD_WELLDEF);
 
 val MUL_EVAL = store_thm("MUL_EVAL",
   `!a b. n2w a * n2w b = n2w (a * b)`,
-  SELECT_WORD_TAC word_mul_def MUL_WELLDEF);
+  QUOTIENT_WORD_TAC word_mul_def MUL_WELLDEF);
 
 val ONE_COMP_EVAL = store_thm("ONE_COMP_EVAL",
   `!a. NOT (n2w a) = n2w (ONE_COMP a)`,
-  SELECT_WORD_TAC word_1comp_def ONE_COMP_WELLDEF);
+  QUOTIENT_WORD_TAC word_1comp_def ONE_COMP_WELLDEF);
 
 val TWO_COMP_EVAL = store_thm("TWO_COMP_EVAL",
   `!a. ~(n2w a) = n2w (TWO_COMP a)`,
-  SELECT_WORD_TAC word_2comp_def TWO_COMP_WELLDEF);
+  QUOTIENT_WORD_TAC word_2comp_def TWO_COMP_WELLDEF);
 
 val WORD_SUB_LT_EQ = store_thm("WORD_SUB_LT_EQ",
   `!a b. b <= a /\ LT_WL b ==> (n2w a - n2w b = n2w (a - b))`,
@@ -1031,46 +1002,46 @@ val WORD_SUB_LT_EQ = store_thm("WORD_SUB_LT_EQ",
 
 val LSR_ONE_EVAL = store_thm("LSR_ONE_EVAL",
   `!a. word_lsr1 (n2w a) = n2w (LSR_ONE a)`,
-  SELECT_WORD_TAC word_lsr1_def LSR_ONE_WELLDEF);
+  QUOTIENT_WORD_TAC word_lsr1_def LSR_ONE_WELLDEF);
 
 val ASR_ONE_EVAL = store_thm("ASR_ONE_EVAL",
   `!a. word_asr1 (n2w a) = n2w (ASR_ONE a)`,
-  SELECT_WORD_TAC word_asr1_def ASR_ONE_WELLDEF
+  QUOTIENT_WORD_TAC word_asr1_def ASR_ONE_WELLDEF
 );
 
 val ROR_ONE_EVAL = store_thm("ROR_ONE_EVAL",
   `!a. word_ror1 (n2w a) = n2w (ROR_ONE a)`,
-  SELECT_WORD_TAC word_ror1_def ROR_ONE_WELLDEF
+  QUOTIENT_WORD_TAC word_ror1_def ROR_ONE_WELLDEF
 );
 
 val RRX_EVAL = store_thm("RRX_EVAL",
   `!a c. RRX c (n2w a) = n2w (RRXn c a)`,
-  SELECT_WORD_TAC RRX_def RRX_WELLDEF
+  QUOTIENT_WORD_TAC RRX_def RRX_WELLDEF
 );
 
 val LSB_EVAL = store_thm("LSB_EVAL",
   `!a. LSB (n2w a) = LSBn a`,
-  SELECT_WORD_TAC LSB_def LSB_WELLDEF
+  QUOTIENT_WORD_TAC LSB_def LSB_WELLDEF
 );
 
 val MSB_EVAL = store_thm("MSB_EVAL",
   `!a. MSB (n2w a) = MSBn a`,
-  SELECT_WORD_TAC MSB_def MSB_WELLDEF
+  QUOTIENT_WORD_TAC MSB_def MSB_WELLDEF
 );
 
 val OR_EVAL = store_thm("OR_EVAL",
-  `!a b. n2w a | n2w b = n2w (OR a b)`,
-  SELECT_WORD_TAC bitwise_or_def OR_WELLDEF
+  `!a b. (n2w a | n2w b) = n2w (OR a b)`,
+  QUOTIENT_WORD_TAC bitwise_or_def OR_WELLDEF
 );
 
 val EOR_EVAL = store_thm("EOR_EVAL",
   `!a b. n2w a # n2w b = n2w (EOR a b)`,
-  SELECT_WORD_TAC bitwise_eor_def EOR_WELLDEF
+  QUOTIENT_WORD_TAC bitwise_eor_def EOR_WELLDEF
 );
 
 val AND_EVAL = store_thm("AND_EVAL",
   `!a b. n2w a & n2w b = n2w (AND a b)`,
-  SELECT_WORD_TAC bitwise_and_def AND_WELLDEF
+  QUOTIENT_WORD_TAC bitwise_and_def AND_WELLDEF
 );
 
 val BITS_EVAL = store_thm("BITS_EVAL",
